working on the proofs for STac.
- What is missing is the well-formedness of substitutions.

theories/STac/Apply.v
@@ -1,5 +1,5 @@
+Require Import ExtLib.Data.Eq.
 Require Import ExtLib.Data.HList.
-Require Import ExtLib.Core.RelDec.
 Require Import ExtLib.Tactics.
 Require Import MirrorCore.EnvI.
 Require Import MirrorCore.SymI.
@@ -16,7 +16,9 @@ Section parameterized.
   Variable typ : Type.
   Variable expr : Type.
   Variable subst : Type.
-  Variable tyProp : typ.
+  Variable RType_typ : RType typ.
+  Variable Typ0_Prop : Typ0 _ Prop.
+  Let tyProp : typ := @typ0 _ _ _ _.
 
   Variable vars_to_uvars : nat -> nat -> expr -> expr.
   Variable exprUnify : tenv typ -> tenv typ -> nat -> expr -> expr -> typ -> subst -> option subst.
@@ -30,22 +32,23 @@ Section parameterized.
     Fixpoint solve_all_but_last
              (es : list expr)
              (sub : subst) {struct es}
-    : Result typ expr subst.
-    refine match es with
-             | nil => @Solved _ _ _ sub
-             | e :: es =>
-               let e := instantiate (fun u => lookup u sub) 0 e in
-               match tac tus tvs sub e with
-                 | Solved sub' => solve_all_but_last es sub'
-                 | More e sub tus tvs =>
-                   match es with
-                     | nil => More e sub tus tvs
-                     | _ => @Fail _ _ _
-                   end
-                 | Fail => @Fail _ _ _
-               end
-           end.
-    Defined.
+    : Result typ expr subst :=
+      match es with
+        | nil => @Solved _ _ _ nil nil sub
+        | e :: es =>
+          let e := instantiate (fun u => lookup u sub) 0 e in
+          match tac tus tvs sub e with
+            | Solved nil nil sub' =>
+              solve_all_but_last es sub'
+            | More tus tvs sub e =>
+              match es with
+                | nil => More tus tvs sub e
+                | _ => @Fail _ _ _
+              end
+            | _ => @Fail _ _ _
+          end
+      end.
+
   End solve_but_last.
 
   Section eapply_other.
@@ -73,27 +76,187 @@ Section parameterized.
         | None => @Fail _ _ _
         | Some sub' =>
           let len_uvars := length tus in
-          let premises := map (vars_to_uvars 0 len_uvars) lem.(premises) in
-          match
-            solve_all_but_last _ (tus ++ lem.(vars)) tvs tac
-                               premises sub'
-          with
-            | Fail => @Fail _ _ _
-            | Solved sub'' =>
-              match pull (expr := expr) len_uvars len_vars sub'' with
-                | None => @Fail _ _ _
-                | Some sub''' => @Solved _ _ _ sub'''
-              end
-            | More tus tvs sub'' e =>
-              (** TODO: In this case it is not necessary to pull everything
-               ** I could leave unification variables in place
+          match pull (expr := expr) len_uvars len_vars sub' with
+            | Some sub'' =>
+              (** If we have instantiated everything then we can be a little
+               ** bit more efficient
                **)
-              match pull (expr := expr) len_uvars len_vars sub'' with
-                | None => @Fail _ _ _
-                | Some sub''' => More (firstn len_uvars tus) tvs sub''' e
+              let premises :=
+                  map (fun e => instantiate (fun u => lookup u sub) 0
+                                            (vars_to_uvars 0 len_uvars e))
+                      lem.(premises)
+              in
+              solve_all_but_last _ tus tvs tac premises sub''
+            | None =>
+              let premises := map (vars_to_uvars 0 len_uvars) lem.(premises) in
+              match
+                solve_all_but_last _ (tus ++ lem.(vars)) tvs tac
+                                   premises sub'
+              with
+                | Fail => @Fail _ _ _
+                | Solved tus' tvs' sub'' =>
+                  match pull (expr := expr) len_uvars len_vars sub'' with
+                    | None => @Fail _ _ _
+                    | Some sub''' => @Solved _ _ _ nil nil sub'''
+                  end
+                | More tus tvs sub'' e =>
+                  (** TODO: In this case it is not necessary to pull everything
+                   ** I could leave unification variables in place
+                   **)
+                  match pull (expr := expr) len_uvars len_vars sub'' with
+                    | None => @Fail _ _ _
+                    | Some sub''' => More (firstn len_uvars tus) tvs sub''' e
+                  end
               end
           end
       end.
   End eapply_other.
+
+
+  Variable Expr_expr : Expr RType_typ expr.
+  Variable ExprOk_expr : ExprOk Expr_expr.
+  Variable Subst_subst : Subst subst expr.
+  Variable SubstOk_subst : @SubstOk _ _ _ _ Expr_expr Subst_subst.
+  Variable SubstUpdate_subst : SubstUpdate subst expr.
+  Variable SubstUpdateOk_subst : SubstUpdateOk SubstUpdate_subst SubstOk_subst.
+  Variable UnifySound_exprUnify : unify_sound _ exprUnify.
+
+  Require Import ExtLib.Data.List.
+  Require Import ExtLib.Structures.Traversable.
+
+  Theorem solve_all_but_last_sound
+  : forall tus tvs (tac : stac typ expr subst) (prems : list expr) (sub : subst),
+      stac_sound tac ->
+      match solve_all_but_last _ tus tvs tac prems sub with
+        | Fail => True
+        | Solved tus' tvs' s' =>
+          match mapT (F := option) (T := list) (goalD Expr_expr Typ0_Prop tus tvs) prems with
+            | Some Gs =>
+              match substD tus tvs sub with
+                | Some sV =>
+                  match substD (tus ++ tus') (tvs ++ tvs') s' with
+                    | Some s'V =>
+                      forall (us : hlist (typD nil) tus)
+                             (vs : hlist (typD nil) tvs),
+                        (exists
+                            (us' : hlist (typD nil) tus')
+                            (vs' : hlist (typD nil) tvs'),
+                            s'V (hlist_app us us') (hlist_app vs vs')) ->
+                        Forall (fun G => G us vs) Gs /\ sV us vs
+                    | None => False
+                  end
+                | None => True
+              end
+            | None => True
+          end
+        | More tus' tvs' s' g' =>
+          match mapT (F := option) (T := list) (goalD Expr_expr Typ0_Prop tus tvs) prems with
+            | Some Gs =>
+              match substD tus tvs sub with
+                | Some sV =>
+                  match goalD Expr_expr Typ0_Prop (tus ++ tus') (tvs ++ tvs') g' with
+                    | Some G' =>
+                      match substD (tus ++ tus') (tvs ++ tvs') s' with
+                        | Some s'V =>
+                          forall (us : hlist (typD nil) tus)
+                                 (vs : hlist (typD nil) tvs),
+                            (exists
+                                (us' : hlist (typD nil) tus')
+                                (vs' : hlist (typD nil) tvs'),
+                                s'V (hlist_app us us') (hlist_app vs vs') /\
+                                G' (hlist_app us us') (hlist_app vs vs')) ->
+                            Forall (fun G => G us vs) Gs /\ sV us vs
+                        | None => False
+                      end
+                    | None => False
+                  end
+                | None => True
+              end
+            | None => True
+          end
+      end.
+  Proof.
+    intros.
+    induction prems.
+    { simpl. forward. admit. }
+    { admit. }
+  Qed.
+
+  Hypothesis vars_to_uvars_spec : forall (tus0 : tenv typ) (e : expr) (tvs0 : list typ)
+     (t : typ) (tvs' : list typ)
+     (val : hlist (typD nil) tus0 ->
+            hlist (typD nil) (tvs0 ++ tvs') -> typD nil t),
+   exprD' tus0 (tvs0 ++ tvs') e t = Some val ->
+   exists
+     val' : hlist (typD nil) (tus0 ++ tvs') ->
+            hlist (typD nil) tvs0 -> typD nil t,
+     exprD' (tus0 ++ tvs') tvs0 (vars_to_uvars (length tvs0) (length tus0) e)
+       t = Some val' /\
+     (forall (us : hlist (typD nil) tus0) (vs' : hlist (typD nil) tvs')
+        (vs : hlist (typD nil) tvs0),
+      val us (hlist_app vs vs') = val' (hlist_app us vs') vs).
+
+  Theorem APPLY_sound
+  : forall lem tac,
+      @lemmaD typ _ expr _ expr (@goalD _ _ _ _ _ ) (@typ0 _ _ _ _)
+              (fun P => match typ0_cast nil in _ = T return T
+                        with
+                          | eq_refl => P
+                        end)
+              nil nil lem ->
+      stac_sound tac ->
+      stac_sound (eapply_other _ _ lem tac).
+  Proof.
+    intros. red. intros.
+    unfold eapply_other.
+    consider (eapplicable tyProp vars_to_uvars exprUnify s tus tvs lem g); auto; intros.
+    eapply (@eapplicable_sound _ _ _ _ _ tyProp (@typ0_cast _ _ _ _)) in H1; eauto.
+    { consider (pull (length tus) (length (vars lem)) s0); intros.
+      { generalize (@solve_all_but_last_sound tus tvs tac
+                      (map
+                         (fun e : expr =>
+                            instantiate (fun u : nat => lookup u s) 0
+                                         (vars_to_uvars 0 (length tus) e)) (premises lem))
+                      s1 H0).
+        match goal with
+          | |- match ?X with _ => _ end -> match ?Y with _ => _ end =>
+            change Y with X; consider X; intros
+        end; auto.
+        { admit. (** Big **) }
+        { admit. (** Big **) } }
+      { generalize (@solve_all_but_last_sound (tus ++ vars lem) tvs tac
+                      (map (vars_to_uvars 0 (length tus)) (premises lem))
+                      s0 H0).
+        match goal with
+          | |- match ?X with _ => _ end -> match match ?Y with _ => _ end with _ => _ end =>
+            change Y with X; consider X; intros
+        end; auto.
+        { admit. (** Big **) }
+        { forward.
+          red in H. simpl in H.
+          forward.
+          destruct H7.
+          unfold goalD in *. forward.
+          inv_all. subst.
+          subst tyProp.
+          assert (lemmaD' Expr_expr
+                          (fun (tus0 tvs0 : tenv typ) (g0 : expr) =>
+                             match typ0_cast nil in (_ = t) return (ResType tus0 tvs0 t) with
+                               | eq_refl => exprD' tus0 tvs0 g0 (typ0 (F:=Prop))
+                             end)
+                          (fun x : typD nil (typ0 (F:=Prop)) =>
+                             match typ0_cast nil in (_ = t) return t with
+                               | eq_refl => x
+                             end) nil nil lem = Some P1).
+          { revert H. clear.
+            unfold lemmaD'. forward.
+            inv_all; subst.
+            unfold ResType.
+            rewrite eq_option_eq. reflexivity. }
+          clear H.
+          specialize (H9 P1 P0 _ H10 eq_refl H6).
+          admit. } } }
+    { admit. (** BUG **) }
+  Qed.
 
 End parameterized.
