theories/STac/Core.v
@@ -1,9 +1,11 @@
+Require Import Coq.Lists.List.
 Require Import ExtLib.Core.RelDec.
 Require Import ExtLib.Tactics.
 Require Import MirrorCore.EnvI.
 Require Import MirrorCore.SymI.
+Require Import MirrorCore.ExprI.
+Require Import MirrorCore.TypesI.
 Require Import MirrorCore.SubstI3.
-Require Import MirrorCore.EProver2.
 
 Set Implicit Arguments.
 Set Strict Implicit.
@@ -16,7 +18,7 @@ Section parameterized.
 
   Inductive Result : Type :=
   | Fail
-  | Solved : subst -> Result
+  | Solved : list typ -> list typ -> subst -> Result
   | More : list typ -> list typ -> subst -> expr -> Result.
 
   Definition stac : Type :=
@@ -24,17 +26,112 @@ Section parameterized.
     list typ -> list typ -> subst -> expr ->
     Result.
 
-  Axiom goalD : forall (tus tvs : list typ) (s : subst) (goal : expr), Prop.
+  Variable RType_typ : RType typ.
+  Variable Expr_expr : Expr RType_typ expr.
+  Variable Typ0_Prop : Typ0 _ Prop.
+  Variable Subst_subst : Subst subst expr.
+  Variable SubstOk_subst : @SubstOk _ _ _ _ Expr_expr Subst_subst.
+
+  Definition goalD (tus tvs : list typ) (goal : expr) : ResType tus tvs Prop :=
+    match exprD' tus tvs goal (@typ0 _ _ _ _) return ResType tus tvs Prop with
+      | None => None
+      | Some val =>
+        Some match typ0_cast nil in _ = T return HList.hlist _ tus -> HList.hlist _ tvs -> T with
+               | eq_refl => val
+             end
+    end.
 
   Definition stac_sound (tac : stac) : Prop
   := forall tus tvs s (g : expr),
        match tac tus tvs s g with
          | Fail => True
-         | Solved s' =>
-           goalD tus tvs s g (* /\ Extends s' s *)
+         | Solved tus' tvs' s' =>
+           match goalD tus tvs g
+               , substD tus tvs s
+           with
+             | Some G , Some sV =>
+               match substD (tus ++ tus') (tvs ++ tvs') s' with
+                 | None => False
+                 | Some s'V =>
+                   forall us vs,
+                     (exists us' vs',
+                        s'V (HList.hlist_app us us') (HList.hlist_app vs vs')) ->
+                     G us vs /\ sV us vs
+               end
+             | _ , _ => True
+           end
          | More tus' tvs' s' g' =>
-           goalD tus' tvs' s' g' ->
-           goalD tus tvs s g
+           match goalD tus tvs g
+               , substD tus tvs s
+           with
+             | Some G , Some sV =>
+               match goalD (tus ++ tus') (tvs ++ tvs') g'
+                   , substD (tus ++ tus') (tvs ++ tvs') s'
+               with
+                 | Some G' , Some s'V =>
+                   forall us vs,
+                     (exists us' vs',
+                           s'V (HList.hlist_app us us') (HList.hlist_app vs vs')
+                        /\ G' (HList.hlist_app us us') (HList.hlist_app vs vs')) ->
+                     G us vs /\ sV us vs
+                 | _ , _ => False
+               end
+             | _ , _ => True
+           end
        end.
 
+  Lemma More_sound
+  : forall tus tvs s g,
+      match goalD tus tvs g with
+        | Some G =>
+          match substD tus tvs s with
+            | Some sV =>
+              match goalD (tus ++ nil) (tvs ++ nil) g with
+                | Some G' =>
+                  match substD (tus ++ nil)%list (tvs ++ nil)%list s with
+                    | Some s'V =>
+                      forall (us : HList.hlist (typD nil) tus)
+                             (vs : HList.hlist (typD nil) tvs),
+                        (exists us' vs' : HList.hlist (typD nil) nil,
+                           s'V (HList.hlist_app us us') (HList.hlist_app vs vs') /\
+                           G' (HList.hlist_app us us') (HList.hlist_app vs vs')) ->
+                        G us vs /\ sV us vs
+                    | None => False
+                  end
+                | None => False
+              end
+            | None => True
+          end
+        | None => True
+      end.
+  Proof.
+    intros.
+    forward.
+    repeat match goal with
+             | |- match ?X with _ => _ end =>
+               consider X; intros
+           end.
+    { destruct H3 as [ ? [ ? ? ] ].
+      rewrite (HList.hlist_eta x) in *.
+      rewrite (HList.hlist_eta x0) in *.
+      do 2 rewrite HList.hlist_app_nil_r in H3.
+      destruct (eq_sym (HList.app_nil_r_trans tus)).
+      destruct (eq_sym (HList.app_nil_r_trans tvs)).
+      rewrite H0 in *.
+      rewrite H1 in *. inv_all; subst.
+      tauto. }
+    { do 2 rewrite List.app_nil_r in H2.
+      congruence. }
+    { do 2 rewrite List.app_nil_r in H1.
+      congruence. }
+  Qed.
+
 End parameterized.
+
+Arguments stac_sound {typ expr subst _ _ _ _ _} _.
+
+Export MirrorCore.EnvI.
+Export MirrorCore.SymI.
+Export MirrorCore.ExprI.
+Export MirrorCore.TypesI.
+Export MirrorCore.SubstI3.
