theories/STac/Idtac.v
@@ -8,11 +8,18 @@ Section parameterized.
   Variable expr : Type.
   Variable subst : Type.
 
-  Definition IDTAC : stac typ expr subst := @More _ _ _.
+  Definition IDTAC : stac typ expr subst :=
+    fun _ _ sub e => @More _ _ _ nil nil sub e.
+
+  Variable RType_typ : RType typ.
+  Variable Expr_expr : Expr RType_typ expr.
+  Variable Typ0_Prop : Typ0 _ Prop.
+  Variable Subst_subst : Subst subst expr.
+  Variable SubstOk_subst : @SubstOk _ _ _ _ Expr_expr Subst_subst.
 
   Theorem IDTAC_sound : stac_sound IDTAC.
   Proof.
-    red; intros; simpl; auto.
+    intros. unfold IDTAC. red. eapply More_sound.
   Qed.
 
 End parameterized.
