theories/STac/Repeat.v
@@ -1,3 +1,4 @@
+Require Import Coq.Lists.List.
 Require Import ExtLib.Data.HList.
 Require Import ExtLib.Core.RelDec.
 Require Import ExtLib.Tactics.
@@ -6,6 +7,7 @@ Require Import MirrorCore.SymI.
 Require Import MirrorCore.SubstI3.
 Require Import MirrorCore.Util.Iteration.
 Require Import MirrorCore.STac.Core.
+Require Import MirrorCore.STac.Idtac.
 
 Set Implicit Arguments.
 Set Strict Implicit.
@@ -19,15 +21,29 @@ Section parameterized.
   : stac typ expr  subst :=
     (fix DO (n : nat) : stac typ expr  subst :=
        match n with
-         | 0 => @More _ _ _
+         | 0 => @IDTAC _ _ _
          | S n =>
            fun tus tvs sub e =>
+             (** This is like THEN, but lazier **)
              match br tus tvs sub e with
-               | Fail => More tus tvs sub e (** Never fails **)
-               | More e sub tus tvs => DO n e sub tus tvs
-               | Solved s => @Solved _ _ _ s
+               | Fail => More nil nil sub e (** Never fails **)
+               | More tus' tvs' sub e =>
+                 match DO n (tus ++ tus') (tvs ++ tvs') sub e with
+                   | More tus'' tvs'' sub e =>
+                     More (tus' ++ tus'') (tvs' ++ tvs'') sub e
+                   | Solved tus'' tvs'' sub =>
+                     @Solved _ _ _ (tus' ++ tus'') (tvs' ++ tvs'') sub
+                   | Fail => More tus' tvs' sub e
+                 end
+               | Solved tus tvs s => @Solved _ _ _ tus tvs s
              end
        end) max.
+
+  Variable RType_typ : RType typ.
+  Variable Expr_expr : Expr RType_typ expr.
+  Variable Typ0_Prop : Typ0 _ Prop.
+  Variable Subst_subst : Subst subst expr.
+  Variable SubstOk_subst : @SubstOk _ _ _ _ Expr_expr Subst_subst.
 
   Theorem REPEAT_sound
   : forall br, stac_sound br ->
@@ -35,12 +51,57 @@ Section parameterized.
                  stac_sound (REPEAT n br).
   Proof.
     induction n; simpl.
-    { red. auto. }
+    { red; intros. eapply IDTAC_sound. }
     { red. intros.
       specialize (H tus tvs s g).
       destruct (br tus tvs s g); auto.
-      red in IHn. specialize (IHn l l0 s0 e).
-      destruct (REPEAT n br l l0 s0 e); auto. }
+      { eapply More_sound. }
+      { specialize (IHn (tus ++ l) (tvs ++ l0) s0 e).
+        destruct (REPEAT n br (tus ++ l) (tvs ++ l0) s0 e); auto.
+        { forward.
+          match goal with
+            | |- match ?X with _ => _ end =>
+              consider X; intros
+          end.
+          { destruct H6 as [ ? [ ? ? ] ].
+            eapply H3; clear H3.
+            exists (fst (HList.hlist_split _ _ x)).
+            exists (fst (HList.hlist_split _ _ x0)).
+            apply and_comm.
+            apply IHn; clear IHn.
+            exists (snd (HList.hlist_split _ _ x)).
+            exists (snd (HList.hlist_split _ _ x0)).
+            do 2 rewrite hlist_app_assoc.
+            do 2 rewrite hlist_app_hlist_split.
+            destruct (eq_sym (app_ass_trans tus l l1)).
+            destruct (eq_sym (app_ass_trans tvs l0 l2)).
+            rewrite H4 in *. inv_all; subst. assumption. }
+        { clear - H4 H5.
+          generalize dependent P3.
+          do 2 rewrite app_ass. intros. congruence. } }
+        { forward.
+          repeat match goal with
+                   | |- match ?X with _ => _ end =>
+                     consider X; intros
+                 end.
+          { destruct H8 as [ ? [ ? ? ] ].
+            eapply H3; clear H3.
+            exists (fst (HList.hlist_split _ _ x)).
+            exists (fst (HList.hlist_split _ _ x0)).
+            apply and_comm.
+            apply IHn; clear IHn.
+            exists (snd (HList.hlist_split _ _ x)).
+            exists (snd (HList.hlist_split _ _ x0)).
+            do 2 rewrite hlist_app_assoc.
+            do 2 rewrite hlist_app_hlist_split.
+            destruct (eq_sym (app_ass_trans tus l l1)).
+            destruct (eq_sym (app_ass_trans tvs l0 l2)).
+            rewrite H4 in *. rewrite H5 in *.
+            inv_all. subst; tauto. }
+          { revert H7 H5.
+            clear. revert P4. do 2 rewrite app_ass. congruence. }
+          { revert H4 H6. clear. revert P3.
+            do 2 rewrite app_ass. congruence. } } } }
   Qed.
 
 End parameterized.
