theories/STac/Simplify.v
@@ -1,3 +1,4 @@
+Require Import ExtLib.Tactics.
 Require Import MirrorCore.STac.Core.
 
 Set Implicit Arguments.
@@ -12,17 +13,55 @@ Section parameterized.
              (f : list typ -> list typ -> subst -> expr -> expr)
   : stac typ expr subst :=
     fun tus tvs s e =>
-      More tus tvs s (f tus tvs s e).
+      More nil nil s (f tus tvs s e).
+
+  Variable RType_typ : RType typ.
+  Variable Expr_expr : Expr RType_typ expr.
+  Variable ExprOk_expr : ExprOk Expr_expr.
+  Variable Typ0_Prop : Typ0 _ Prop.
+  Variable Subst_subst : Subst subst expr.
+  Variable SubstOk_subst : @SubstOk _ _ _ _ Expr_expr Subst_subst.
 
   Theorem SIMPLIFY_sound
   : forall f,
       (forall tus tvs s e e',
          f tus tvs s e = e' ->
-         goalD tus tvs s e' -> goalD tus tvs s e) ->
+         match @goalD _ _ _ Expr_expr _ tus tvs e
+             , @substD _ _ _ _ Expr_expr _ _ tus tvs s
+             , @goalD _ _ _ _ _ tus tvs e'
+         with
+           | None , _ , _ => True
+           | _ , None , _ => True
+           | Some _ , Some _ , None => False
+           | Some eD , Some sD , Some eD' =>
+             forall us vs,
+               sD us vs ->
+               eD us vs <-> eD' us vs
+         end) ->
       stac_sound (SIMPLIFY f).
   Proof.
     intros. unfold stac_sound, SIMPLIFY.
-    intros. eapply H. reflexivity. eauto.
+    intros.
+    specialize (H tus tvs s g _ eq_refl).
+    forward.
+    repeat match goal with
+             | |- match ?X with _ => _ end =>
+               consider X; intros
+           end.
+    { destruct H5 as [ ? [ ? ? ] ].
+      rewrite (HList.hlist_eta x) in *.
+      rewrite (HList.hlist_eta x0) in *.
+      do 2 rewrite HList.hlist_app_nil_r in H5.
+      specialize (H2 us vs).
+      destruct (eq_sym (HList.app_nil_r_trans tus)).
+      destruct (eq_sym (HList.app_nil_r_trans tvs)).
+      rewrite H4 in *.
+      rewrite H3 in *. inv_all; subst.
+      intuition. }
+    { clear - H4 H0.
+      do 2 rewrite List.app_nil_r in *. congruence. }
+    { clear - H3 H1.
+      do 2 rewrite List.app_nil_r in *. congruence. }
   Qed.
 
 End parameterized.
