theories/STac/Solve.v
@@ -11,9 +11,16 @@ Section parameterized.
   Definition SOLVE (b : stac typ expr subst) : stac typ expr subst :=
     fun e sub tus tvs =>
       match b e sub tus tvs with
-        | Solved s => @Solved _ _ _ s
+        | Solved tus tvs s => @Solved _ _ _ tus tvs s
         | x => @Fail _ _ _
       end.
+
+  Variable RType_typ : RType typ.
+  Variable Expr_expr : Expr RType_typ expr.
+  Variable ExprOk_expr : ExprOk Expr_expr.
+  Variable Typ0_Prop : Typ0 _ Prop.
+  Variable Subst_subst : Subst subst expr.
+  Variable SubstOk_subst : @SubstOk _ _ _ _ Expr_expr Subst_subst.
 
   Theorem SOLVE_sound : forall t, stac_sound t -> stac_sound (SOLVE t).
   Proof.
