theories/STac/Then.v
@@ -1,3 +1,5 @@
+Require Import Coq.Lists.List.
+Require Import ExtLib.Tactics.
 Require Import MirrorCore.STac.Core.
 
 Set Implicit Arguments.
@@ -9,13 +11,25 @@ Section parameterized.
   Variable subst : Type.
 
   Definition THEN (a b : stac typ expr subst) : stac typ expr subst :=
-    fun e sub tus tvs =>
-      let res := a e sub tus tvs in
+    fun tus tvs sub e =>
+      let res := a tus tvs sub e in
       match res with
-        | Solved s => @Solved _ _ _ s
-        | More e sub tus tvs => b e sub tus tvs
+        | Solved tus tvs s => @Solved _ _ _ tus tvs s
+        | More tus' tvs' sub e =>
+          match b (tus ++ tus') (tvs ++ tvs') sub e with
+            | Solved tus'' tvs'' sub => @Solved _ _ _ (tus' ++ tus'') (tvs' ++ tvs'') sub
+            | More tus'' tvs'' sub e => More (tus' ++ tus'') (tvs' ++ tvs'') sub e
+            | Fail => @Fail _ _ _
+          end
         | Fail => res
       end.
+
+  Variable RType_typ : RType typ.
+  Variable Expr_expr : Expr RType_typ expr.
+  Variable ExprOk_expr : ExprOk Expr_expr.
+  Variable Typ0_Prop : Typ0 _ Prop.
+  Variable Subst_subst : Subst subst expr.
+  Variable SubstOk_subst : @SubstOk _ _ _ _ Expr_expr Subst_subst.
 
   Theorem THEN_sound
   : forall a b, stac_sound a -> stac_sound b -> stac_sound (THEN a b).
@@ -23,8 +37,54 @@ Section parameterized.
     unfold stac_sound, THEN; intros.
     specialize (H tus tvs s g).
     destruct (a tus tvs s g); auto.
-    specialize (H0 l l0 s0 e).
-    destruct (b l l0 s0 e); auto.
+    specialize (H0 (tus ++ l) (tvs ++ l0) s0 e).
+    destruct (b (tus ++ l) (tvs ++ l0) s0 e); auto.
+    { forward.
+      match goal with
+        | |- match ?X with _ => _ end =>
+          consider X; intros
+      end.
+      { destruct H7 as [ ? [ ? ? ] ].
+        eapply H4; clear H4.
+        exists (fst (HList.hlist_split _ _ x)).
+        exists (fst (HList.hlist_split _ _ x0)).
+        eapply and_comm.
+        eapply H5; clear H5.
+        exists (snd (HList.hlist_split _ _ x)).
+        exists (snd (HList.hlist_split _ _ x0)).
+        do 2 rewrite HList.hlist_app_assoc.
+        do 2 rewrite HList.hlist_app_hlist_split.
+        repeat match goal with
+                 | |- context [ match ?X with _ => _ end ] =>
+                   destruct X
+               end.
+        rewrite H3 in *. inv_all; subst. assumption. }
+      { intros. revert H3 H6.
+        clear - P3. revert P3.
+        do 2 rewrite app_ass. intros. congruence. } }
+    { forward.
+      repeat match goal with
+               | |- match ?X with _ => _ end =>
+                 consider X; intros
+             end.
+      { forward_reason.
+        eapply H4; clear H4.
+        exists (fst (HList.hlist_split _ _ x)).
+        exists (fst (HList.hlist_split _ _ x0)).
+        eapply and_comm.
+        eapply H6; clear H6.
+        exists (snd (HList.hlist_split _ _ x)).
+        exists (snd (HList.hlist_split _ _ x0)).
+        do 2 rewrite HList.hlist_app_assoc.
+        do 2 rewrite HList.hlist_app_hlist_split.
+        destruct (eq_sym (HList.app_ass_trans tus l l1)).
+        destruct (eq_sym (HList.app_ass_trans tvs l0 l2)).
+        rewrite H3 in *. rewrite H8 in *. inv_all; subst.
+        split; assumption. }
+      { revert H5 H8. clear. revert P4.
+        do 2 rewrite app_ass. congruence. }
+      { revert H7 H3. clear. revert P3.
+        do 2 rewrite app_ass. congruence. } }
   Qed.
 
 End parameterized.
