theories/STac/Try.v
@@ -11,15 +11,23 @@ Section parameterized.
   Definition TRY (b : stac typ expr subst) : stac typ expr subst :=
     fun tus tvs sub e =>
       match b tus tvs sub e with
-        | Fail => More tus tvs sub e
+        | Fail => More nil nil sub e
         | x => x
       end.
+
+  Variable RType_typ : RType typ.
+  Variable Expr_expr : Expr RType_typ expr.
+  Variable ExprOk_expr : ExprOk Expr_expr.
+  Variable Typ0_Prop : Typ0 _ Prop.
+  Variable Subst_subst : Subst subst expr.
+  Variable SubstOk_subst : @SubstOk _ _ _ _ Expr_expr Subst_subst.
 
   Theorem TRY_sound : forall b, stac_sound b -> stac_sound (TRY b).
   Proof.
     unfold stac_sound; intros.
     specialize (H tus tvs s g). unfold TRY.
     destruct (b tus tvs s g); auto.
+    eapply More_sound.
   Qed.
 
 End parameterized.
